prove lemmas on isa level

model/agp32RelationScript.sml
@@ -35,28 +35,33 @@ End
 (* software conditions *)
 (* self modified: a memory write operation does not affect the fetched value of the next 3 instructions *)
 Definition SC_self_mod_isa_def:
-  SC_self_mod_isa (a:ag32_state) (n:num) <=>
-  is_wrMEM_isa (FUNPOW Next (n-1) a) ==> 
-  !i. i > n /\ i < n + 4 /\ (FUNPOW Next (i-1) a).PC <> mem_data_addr (FUNPOW Next (n-1) a)
+  SC_self_mod_isa (a:ag32_state) <=>
+  !n i. is_wrMEM_isa (FUNPOW Next (n-1) a) ==> 
+  i > n /\ i < n + 4 ==> align_addr (FUNPOW Next (i-1) a).PC <> align_addr (dataB (FUNPOW Next (n-1) a))
 End  
 
 Definition SC_self_mod_def:
   SC_self_mod (I:num # num -> num option) (a:ag32_state) <=> 
   !t j. j = THE (I (2,t)) \/ j = THE (I (3,t)) \/ j = THE (I (4,t)) ==>
   is_wrMEM_isa (FUNPOW Next (j-1) a) ==>
-  mem_data_addr (FUNPOW Next (j-1) a) <> (FUNPOW Next (THE (I (1,t)) -1) a).PC
+  align_addr (dataB (FUNPOW Next (j-1) a)) <> align_addr (FUNPOW Next (THE (I (1,t)) -1) a).PC
 End
 
 (* on ISA level
-isa_self_mod ==> this one
-SC_self_mod I a <=> try with ISA only
-!t.j = I (2,t) \/ j = I (3,t) \/ j = I (4,t) ==> 
-   is_wrMEM_isa (FUNPOW Next (j-1) a) ==>
-   j < I (1,t) ==>
-   wr_mem_addr (FUNPOW Next (j-1) a) <> (FUNPOW Next (I(1,t)-1) a).PC
+SC_self_mod_isa ==> SC_self_mod
+
 lemma
-!adr a n.
-SC_self_mod_isa a n ==> value_at_addr adr (FUNPOW Next n a).MEM = value_at_addr adr (FUNPOW Next (i-1) a).MEM
+!a n i.
+is_wrMEM_isa (FUNPOW Next (n-1) a) ==> 
+i > n /\ i < n + 4 ==> (FUNPOW Next (i-1) a).PC <> mem_data_addr (FUNPOW Next (n-1) a) ==> 
+value_at_addr (FUNPOW Next (i-1) a).PC (FUNPOW Next i-1 a).MEM = value_at_addr (FUNPOW Next (i-1) a).PC (FUNPOW Next n a).MEM
+
+!I a t j.
+j = THE (I (2,t)) \/ j = THE (I (3,t)) \/ j = THE (I (4,t)) ==>
+is_wrMEM_isa (FUNPOW Next (j-1) a) ==>
+mem_data_addr (FUNPOW Next (j-1) a) <> (FUNPOW Next (THE (I (1,t)) -1) a).PC ==> 
+value_at_addr (FUNPOW Next (THE (I (1,t)) -1) a).PC (FUNPOW Next (THE (I (1,t)) -1) a).MEM = 
+value_at_addr (FUNPOW Next (THE (I (1,t)) -1) a).PC (FUNPOW Next (THE (I (4,t))) a).MEM
 *)
 
 (* Definitions of relations to prove the correctness of the pipelined Silver *)
